Anf kind of works

Anf.v
@@ -5,11 +5,9 @@ From STLCZK Require Import Stlc.
 From STLCZK Require Import R1cs.
 From STLCZK Require Import Ltac.
 
-Require Import Coq.Vectors.VectorDef.
-Require Import ExtLib.Structures.Monads.
-Require Import ExtLib.Data.Monads.StateMonad.
-Require Import Coq.Init.Nat.
-
+From Coq Require Import Vectors.VectorDef.
+From Coq Require Import Init.Nat.
+From Coq Require Import Lists.List.
 
 Generalizable All Variables.
 
@@ -18,96 +16,173 @@ Module Anf(PF: GaloisField).
   Include Stlc PF.
   Import ListNotations.
   Local Open Scope nat_scope.
-
-  Definition var := nat.
   
   Inductive anfexp : Set :=
-  | Let(n: var)(l: cexp)(e: exp)
-  | Cexp(e: cexp)
-  | Aexp(e: aexp)
-  with cexp: Set :=
-  | App(f: aexp)(v: aexp)
-  | If(c: aexp)(t: cexp)(e: cexp)
+  | Let(l: aexp)(e: anfexp)
+  | Value(v: value)
+  with value: Set :=
+  | CField(f: Fp)
+  | Var_f(s: var)
+  | CBoolean(b: bool)
+  | Var_b(v: nat)
+  | Lambda(e: anfexp)
   with aexp: Set :=
-  | Num(f: Fp)
-  | Boolean(b: bool)
-  | Var(v: var)
-  | Primop(o: op) (l: aexp) (r: aexp)
-  | Eq(l: aexp)(r: aexp)
-  | Not(l: aexp)
-  | Lambda(i: nat) (e: exp).
+  | App(f: value)(v: value)
+  | Select(c: value)(t: value)(e: value)
+  | Primop(o: op) (l: value) (r: value)
+  | Eq(l: value)(r: value)
+  | Not(l: value).
 
-  Definition is_primop(e: exp): bool :=
+  Fixpoint subst_anfexp(e: anfexp)(n: nat)(val: value): anfexp :=
     match e with
-    | tm_binop a op b =>
-      if is_value_of_exp a && is_value_of_exp b then
-        true
-      else
-        false
-    | tm_eq a b =>
-      if is_value_of_exp a && is_value_of_exp b then
-        true
-      else
-        false
-    | _ => false
-    end.
+    | Let l e => Let (subst_aexp l n val) (subst_anfexp e n val)
+    | Value v => Value (subst_value v n val)
+    end
+  with subst_value(e: value)(v: nat)(val: value): value :=
+         match e with
+         | Var_b b => if b =? v then val else Var_b b
+         | Lambda e => Lambda (subst_anfexp e v val)
+         | o => o
+         end
+  with subst_aexp(e: aexp)(v: nat)(val: value): aexp :=
+         match e with
+         | App f a => App (subst_value f v val) (subst_value a v val)
+         | Select c t e => Select (subst_value c v val)
+                                 (subst_value t v val)
+                                 (subst_value e v val)
+         | Primop o l r => Primop o
+                                 (subst_value l v val)
+                                 (subst_value r v val)
+         | Eq l r => Eq (subst_value l v val)
+                       (subst_value r v val)
+         | Not l => Not (subst_value l v val)
+         end.
 
-  Definition max_binder(e: exp): nat :=
-    let fix max_binder_list e' :=
-      match e' with
-      | tm_var_b n => [n]
-      | tm_var_f x => []
-      | tm_abs _ e => max_binder_list e
-      | tm_app l r => max_binder_list l ++ max_binder_list r
-      | tm_let l r => max_binder_list l ++ max_binder_list r
-      | tm_constant _ => []
-      | tm_binop l _ r => max_binder_list l ++ max_binder_list r
-      | tm_eq l r => max_binder_list l ++ max_binder_list r
-      | tm_not e => max_binder_list e
-      | tm_ifthenelse e l r =>
-        max_binder_list e ++ max_binder_list l ++ max_binder_list r
-      end in
-    let fix list_max l n := match l with
-                            | [] => n
-                            | h:: ts => if n <? h then list_max ts h else list_max ts n
-                            end in
-    list_max (max_binder_list e) 0.
+  Fixpoint shift_aexp(e: aexp)(v: nat): aexp :=
+    match e with
+    | App f a => App (shift_value f v) (shift_value a v)
+    | Select c t e => Select (shift_value c v)
+                            (shift_value t v)
+                            (shift_value e v)
+    | Primop o l r => Primop o
+                            (shift_value l v)
+                            (shift_value r v)
+    | Eq l r => Eq (shift_value l v)
+                  (shift_value r v)
+    | Not l => Not (shift_value l v)
+    end
+  with shift_anfexp(e: anfexp)(n: nat): anfexp :=
+    match e with
+    | Let l e => Let (shift_aexp l n) (shift_anfexp e n)
+    | Value v => Value (shift_value v n)
+    end
+  with shift_value(e: value)(v: nat): value :=
+         match e with
+         | Var_b b => Var_b (b + v)
+         | Lambda e => Lambda (shift_anfexp e v)
+         | o => o
+         end.
   
-  Fixpoint normalize (e: exp)(k: anfexp -> anfexp): anfexp :=
+  Fixpoint binders_aexp(e: aexp): list nat :=
     match e with
-    | tm_abs _ body => k (Lambda (max_binder body) (normalize-term body))
-    | tm_let m1 m2 =>
-      normalize m1
-                (fun n1 =>
-                   Let (max_binder e) n1 (normalize m2 k))
-    | tm_ifthenelse m1 m2 m3 =>
-      normalize-name m1 (fun t =>
-                           k (If t (normalize-term m2) (normalize-term m3)))
-    | tm_binop m1 op m2 =>
-      if is_primop e then
-        normalize-name m1 (fun t1 =>
-                             normalize-name m2 (fun t2 =>
-                                                  k (Primop op t1 t2)))
-      else
-        normalize m1 (fun t1 =>
-                        normalize m2 (fun t2 =>
-                                        k (Primop t1 t2))) (** TODO: This is not an aexp *)
-    | tm_app m1 m2 =>
-      normalize m1 (fun t1 =>
-                      normalize m2 (fun t2 =>
-                                      k (App t1 t2)))
-    | tm_eq m1 m2 =>
-       if is_primop e then
-        normalize-name m1 (fun t1 =>
-                             normalize-name m2 (fun t2 =>
-                                                  k (Eq op t1 t2)))
-      else
-        normalize m1 (fun t1 =>
-                        normalize m2 (fun t2 =>
-                                        k (Eq t1 t2))) (** TODO: This is not an aexp *)
-    | tm_not e => normalize e (fun t =>
-                                k (Not t))
-    | value => k (
+    | App f a => binders_value f ++ binders_value a
+    | Select c t e => binders_value c ++ binders_value t ++ binders_value e
+    | Primop o l r => binders_value l ++ binders_value r
+    | Eq l r => binders_value l ++ binders_value r
+    | Not l => binders_value l
+    end
+  with binders_anfexp(e: anfexp): list nat :=
+    match e with
+    | Let l e => binders_aexp l ++ binders_anfexp e
+    | Value v => binders_value v
+    end
+  with binders_value(e: value): list nat :=
+         match e with
+         | Var_b b => [b]
+         | o => []
+         end.
+
+  Definition shift(n: nat)(l: list aexp): list aexp :=
+    map (fun e => shift_aexp e n) l.
+  
+  Definition max_binder(e: list aexp): nat :=
+    list_max (flat_map binders_aexp e).
+
+  Fixpoint substitute(n: nat)(v: value)(l: list aexp): list aexp :=
+    match l with
+    | [] => []
+    | h :: ts => subst_aexp h n v :: substitute (S n) (shift_value v 1) ts
+    end.
+  
+  Fixpoint anf_translate (e: exp): anfexp :=
+    let fix make_lets(l: list aexp)(v: value): anfexp :=
+        match l with
+        | [] => Value v
+        | h :: ts => Let h (make_lets ts v)
+        end in
+    let fix translate_helper(e: exp): (list aexp * value) :=
+        match e with
+        | tm_var_b n => ([], Var_b n)
+        | tm_var_f x => ([], Var_f x)
+        | tm_abs _ e => ([], Lambda (anf_translate e))
+        | tm_app e1 e2 =>
+          let (es1, v1) := translate_helper e1 in
+          let (es2, v2) := translate_helper e2 in
+          let n := length es1 in
+          let m := length es2 in
+          (es1 ++ shift n es2 ++ [App (shift_value v1 m) v2], Var_b 0)
+        | tm_let e1 e2 =>
+          let (es1, v1) := translate_helper e1 in
+          let (es2, v2) := translate_helper e2 in
+          let n := length es1 in
+          let m := length es2 in
+          (es1 ++ (substitute 0 v1 es2), v2)
+        | tm_constant (const_field f) => ([], CField f)
+        | tm_constant (const_bool b) => ([],  CBoolean b)
+        | tm_binop e1 op e2 =>
+          let (es1, v1) := translate_helper e1 in
+          let (es2, v2) := translate_helper e2 in
+          let n := length es1 in
+          let m := length es2 in
+          (es1 ++ shift n es2 ++ [Primop op (shift_value v1 m) v2], Var_b 0)
+        | tm_eq e1 e2 =>
+          let (es1, v1) := translate_helper e1 in
+          let (es2, v2) := translate_helper e2 in
+          let n := length es1 in
+          let m := length es2 in
+          (es1 ++ shift n es2 ++ [Eq (shift_value v1 m) v2], Var_b 0)
+        | tm_not e =>
+          let (es, v) := translate_helper e in
+          (es ++ [Not v], Var_b 0)
+        | tm_ifthenelse c e1 e2 =>
+          let (ce, vc) := translate_helper c in
+          let (es1, v1) := translate_helper e1 in
+          let (es2, v2) := translate_helper e2 in
+          let size_ce := length ce in
+          let size_es1 := length es1 in
+          let size_es2 := length es2 in
+          (ce ++ shift size_ce es1 ++ shift (size_ce + size_es1) es2 ++
+              [Select (
+                   shift_value vc (size_es1 + size_es2)) (shift_value v1 size_es2) v2], Var_b 0)
+        end in
+    let (defs, ans) := translate_helper e in
+    make_lets defs ans.
+
+  Definition foo :=
+    <{ \_: Bool,
+           let #0 && #0 in
+           let #0 || #1 in
+           #0 || #0 }>.
+
+  Definition bar :=
+    <{ \_: Bool,
+           let #0 || #0 in
+           if #0 then #1 else #1 && #1
+     }>.
+             
+    Compute anf_translate bar.
+
+End Anf.
       
         
                     
