NonEmpty.v
@@ -1,0 +1,148 @@
+Set Implicit Arguments.
+Unset Strict Implicit.
+Unset Printing Implicit Defensive.
+      
+(** ** NonEmpty lists *)
+Require Import Coq.Lists.List.
+Import ListNotations.
+Require Import Coq.Arith.PeanoNat.
+Local Open Scope nat_scope.
+Require Import Coq.micromega.Lia.
+
+Inductive NonEmpty (a : Type) : Type :=
+  | NE_Sing : a -> NonEmpty a
+  | NE_Cons : a -> NonEmpty a -> NonEmpty a.
+
+Arguments NE_Sing [_] _.
+Arguments NE_Cons [_] _ _.
+
+Fixpoint NE_from_list {a} (x : a) (xs : list a) : NonEmpty a :=
+  match xs with
+    | nil => NE_Sing x
+    | cons y ys => NE_Cons x (NE_from_list y ys)
+  end.
+
+Fixpoint NE_length {a} (ne : NonEmpty a) : nat :=
+  match ne with
+    | NE_Sing x => 1
+    | NE_Cons x xs => 1 + NE_length xs
+  end.
+
+Fixpoint NE_to_list {a} (ne : NonEmpty a) : list a :=
+  match ne with
+    | NE_Sing x => cons x nil
+    | NE_Cons x xs => cons x (NE_to_list xs)
+  end.
+
+Coercion NE_to_list : NonEmpty >-> list.
+
+Lemma NE_to_list_from_list {a} : forall (x : a) xs,
+  NE_to_list (NE_from_list x xs) = x :: xs.
+Proof.
+  intros x xs.
+  generalize dependent x.
+  induction xs; cbn; try reflexivity.
+  - rewrite IHxs; intros; reflexivity.
+Defined.
+
+Definition NE_head {a} (ne : NonEmpty a) : a :=
+  match ne with
+    | NE_Sing x => x
+    | NE_Cons x _ => x
+  end.
+Fixpoint NE_last {a} (ne : NonEmpty a) : a :=
+  match ne with
+    | NE_Sing x => x
+    | NE_Cons x xs => NE_last xs
+  end.
+Fixpoint NE_tail a (ne : NonEmpty a) : list a :=
+  match ne with
+    | NE_Sing x => [x]
+    | NE_Cons x xs => x :: NE_tail xs
+  end.
+
+Fixpoint NE_app a (na: NonEmpty a)(nb: NonEmpty a): NonEmpty a :=
+  match na with
+  | NE_Cons h ts => NE_Cons h (NE_app ts nb)
+  | NE_Sing a => NE_Cons a nb
+  end.
+
+Fixpoint NE_map a b (f:a -> b)(na: NonEmpty a): NonEmpty b :=
+  match na with
+  | NE_Cons h ts => NE_Cons (f h) (NE_map f ts)
+  | NE_Sing a => NE_Sing (f a)
+  end.
+
+Lemma NE_length_gt_0: forall s (l: NonEmpty s),
+    NE_length l > 0.
+  intros. induction l; cbn; lia.
+Defined.
+
+(** NonEmpty nat *)
+Fixpoint NE_max (na: NonEmpty nat): nat :=
+  match na with
+  | NE_Cons h ts => if (NE_max ts) <? h then h else (NE_max ts)
+  | NE_Sing a => a
+  end.
+
+Lemma NE_max_cons_h: forall h ts,
+  NE_max ts <= h ->
+  NE_max (NE_Cons h ts) = h.
+Proof.
+  intros; destruct h.
+  - inversion H.
+    cbn.
+    rewrite H1.
+    reflexivity.
+  - cbn.
+    destruct (Nat.leb_spec0 (NE_max ts) h).
+    + reflexivity.
+    + inversion H.
+      reflexivity.      
+      apply n in H1.
+      contradiction.
+Defined.
+
+Lemma NE_max_cons_ts: forall h ts,
+  h <= NE_max ts ->
+  NE_max (NE_Cons h ts) = NE_max ts.
+Proof.
+  intros; destruct h.
+  - reflexivity.
+  - cbn.
+    destruct (NE_max ts <=? h) eqn:Hn.
+    rewrite Nat.leb_le in Hn.
+    lia.
+    reflexivity.
+Defined.
+
+Lemma NE_max_cons: forall h ts i,
+    NE_max (NE_Cons h ts) <= i ->
+    h <= i /\ NE_max ts <= i.
+Proof.
+  intros.
+  assert(Hnot: forall a b, ~ a <= b -> b < a) by lia.
+  destruct (Nat.le_decidable (NE_max ts) h); split.
+  - pose proof (NE_max_cons_h H0).
+    rewrite H1 in H.
+    assumption.
+  - pose proof (NE_max_cons_h H0).
+    rewrite H1 in H.
+    exact (Nat.le_trans _ _ _ H0 H).
+Admitted.
+
+Lemma NE_max_sing: forall v i,
+    NE_max (NE_Sing v) <= i ->
+    v <= i.
+  intros; cbn in *; assumption.
+Defined.
+
+Lemma NE_map_cons: forall a b (f: a -> b) h ts,
+  NE_map f (NE_Cons h ts) = NE_Cons (f h) (NE_map f ts).
+  intros; cbn; reflexivity.
+Defined.
+
+Lemma NE_map_sing: forall a b (f: a -> b) v,
+    NE_map f (NE_Sing v) = NE_Sing (f v).
+  intros; cbn; reflexivity.
+Defined.
