Stlc.v
@@ -33,7 +33,8 @@ Module Stlc_Ott(Import PF: GaloisField.GaloisField).
   Inductive constant : Set := 
   | const_bool (b5:bool)
   | const_field (n5:Fp).
-  
+
+  (* exp -> anfexp -> (normalization) -> anfexp *)
   Inductive exp : Set := 
   | tm_var_b (_:nat)
   | tm_var_f (x:expvar)
